

## Leibniz' Rule

$$\frac{d}{dx} \int_{u(x)}^{v(x)} f(x, t) dt = f(x, v(x)) \frac{dv}{dx} - f(x, u(x)) \frac{du}{dx} + \int_{u(x)}^{v(x)} \frac{\partial f(x, t)}{\partial x} dt$$

$$\begin{aligned}
& \frac{d}{dx} \int_{t=1/x}^{2/x} \frac{\sin xt}{t} dt \\
&= \frac{\sin 2}{2/x} \cdot -\frac{2}{x^2} - \frac{\sin 1}{1/x} \cdot -\frac{1}{x^2} + \int_{t=1/x}^{2/x} \cos xt \, dt \\
&= -\frac{\sin 2}{x} + \frac{\sin 1}{x} + \left[ \frac{\sin xt}{x} \right]_{t=1/x}^{2/x} \\
&= -\frac{\sin 2}{x} + \frac{\sin 1}{x} + \left( \frac{\sin 2}{x} - \frac{\sin 1}{x} \right) = 0
\end{aligned}$$

$$s = \int_u^v \frac{1 - e^{-t}}{t} dt$$

$$\frac{\partial s}{\partial v} = \frac{1 - e^v}{v} \xrightarrow{v \rightarrow -\infty} \frac{-e^v}{1} \rightarrow -1$$

$$\frac{\partial s}{\partial u} = -\frac{1 - e^u}{u} \xrightarrow{u \rightarrow -\infty} \frac{+e^u}{1} \rightarrow +1$$

**Evaluate the integral**

$$F(\alpha) = \int_0^1 \frac{x^\alpha - 1}{\ln x} dx \quad (\alpha \geq 0)$$

**by differentiating under the integral sign**

Differentiate both sides with respect to  $\alpha$ :

$$\begin{aligned} F'(\alpha) &= \int_0^1 \frac{\partial}{\partial \alpha} \left( \frac{x^\alpha - 1}{\ln x} \right) dx \\ &= \int_0^1 \frac{1}{\ln x} x^\alpha \ln x dx = \int_0^1 x^\alpha dx = \left[ \frac{x^{\alpha+1}}{\alpha+1} \right]_0^1 = \frac{1}{1+\alpha} \end{aligned}$$

Integrating now with respect to  $\alpha$  we obtain  $F(\alpha) = \ln(1 + \alpha) + C$ .

Since  $F(0) = 0, C = 0 \Rightarrow \underline{F(\alpha) = \ln(1 + \alpha)}$

**Evaluate the integral**

$$F(\alpha) = \int_0^\infty e^{-x} \cdot \frac{\sin \alpha x}{x} dx$$

Differentiate both sides with respect to  $\alpha$ :

**Using**  $\int_0^\infty e^{-x^2} = \frac{\sqrt{\pi}}{2}$ , **show that**  $I = \int_0^\infty e^{-x^2} \cos \alpha x \, dx = \frac{\sqrt{\pi}}{2} e^{-\alpha^2/4}$

Differentiate both sides with respect to  $\alpha$ :

$$\frac{dI}{d\alpha} = \int_0^\infty e^{-x^2} \cdot (-x \sin \alpha x) \, dx$$

Integrate “by parts” with  $u = \sin \alpha x, dv = -xe^{-x^2} dx \Rightarrow du = \alpha \cos \alpha x \, dx, v = -e^{-x^2}/2$ :

$$= \left[ -\frac{1}{2} e^{-x^2} \sin \alpha x \right]_0^\infty + \frac{1}{2} \int_0^\infty e^{-x^2} \alpha \cos \alpha x \, dx$$

The first term approaches zero at both limits and the integral is the original integral  $I$  multiplied by  $\alpha$ :

$$\frac{dI}{d\alpha} = \frac{\alpha}{2} I$$

We might recognize this differential equation in the form  $\frac{dy}{dx} = \frac{xy}{2} \Rightarrow \frac{dy}{y} = \frac{1}{2} x \, dx \Rightarrow \ln y = \frac{1}{4} x^2 + C \Rightarrow y = C e^{x^2/4}$ . Thus  $I = C e^{-\alpha^2/4}$  and at  $\alpha = 0$  the given value yields  $C = \sqrt{\pi}/2$  so:

$$\underline{\int_0^\infty e^{-x^2} \cos \alpha x \, dx = \frac{\sqrt{\pi}}{2} e^{-\alpha^2/4}}$$